theories/examples/compression/buffers_laws.v
@@ -26,65 +26,62 @@ Section Specs.
     1: by cbn.
     iModIntro. iFrame "HGC".
     iExists _. iSplitL.
-    { iExists ℓML, _, fid, γfgn. unfold named.
+    { iExists ℓML, _, γfgn. unfold named.
       iSplit; first done. iFrame "HℓbufML".
       iExists vcontent.
-      unfold named. by iFrame "Hγfgnpto Hℓbuf Hγfgnsim HContent". }
+      unfold named. by iFrame "Hγfgnpto Hℓbuf HContent". }
     { cbn. iExists _, _, _. iSplitL; first done.
       iFrame "Hγbuf".
       iSplitL; first (iExists _; iSplit; done).
       iExists _, _, _. iSplit; first done.
-      iFrame "Hγaux". iSplit; first done.
-      iExists _; iSplit; done. }
+      iFrame "Hγaux". iSplit; done. }
   Qed.
 
   Lemma bufToC v ℓbuf Pb c lv θ:
       GC θ
    -∗ isBufferRecordML v ℓbuf Pb c
    -∗ lv ~~ v
-  ==∗ GC θ ∗ isBufferRecord lv ℓbuf Pb c ∗ ∃ (ℓML:loc) fid, ⌜v = (ML_lang.LitV ℓML, (ML_lang.LitV c, ML_lang.LitV (LitForeign fid)))%MLV⌝.
+  ==∗ GC θ ∗ isBufferRecord lv ℓbuf Pb c ∗ ∃ (ℓML:loc) γ, ⌜v = (ML_lang.LitV ℓML, (ML_lang.LitV c, ML_lang.LitV (LitForeign γ)))%MLV⌝.
   Proof.
     iIntros "HGC H Hsim". iNamed "H". iNamed "Hbuf".
-    iDestruct "Hsim" as "#(%γ&%&%&->&Hγbuf&(%γref&->&Hsim)&%γaux&%&%&->&Hγaux&->&%γfgn2&->&Hγfgnsim2)".
-    iPoseProof (lloc_own_foreign_inj with "Hγfgnsim2 Hγfgnsim [$]") as "(HGC&%Hiff)".
-    destruct Hiff as [_ ->]; last done.
+    iDestruct "Hsim" as "#(%γ&%&%&->&Hγbuf&(%γref&->&Hsim)&%γaux&%&%&->&Hγaux&->&->)".
     iMod (ml_to_mut with "[$HGC $HℓbufML]") as "(HGC&(%ℓvs&%γref2&Hγusedref&#Hsim2&#Hγrefsim))".
     iPoseProof (lloc_own_pub_inj with "Hsim2 Hsim [$]") as "(HGC&%Hiff)".
     destruct Hiff as [_ ->]; last done.
     iModIntro. iFrame "HGC". iSplit; last by repeat iExists _. 
-    iExists _, _, _, _, _, _. unfold named.
+    iExists _, _, _, _, _. unfold named.
     iSplit; first done.
     iFrame "Hγbuf". iFrame "Hγaux".
     iSplitL "Hγusedref".
     { destruct ℓvs as [|ℓvs [|??]]; cbn; try done.
       all: iDestruct "Hγrefsim" as "[-> ?]"; try done. }
-    { cbn. iExists _. unfold named. iFrame "Hγfgnpto Hγfgnsim Hℓbuf HContent".
+    { cbn. iExists _. unfold named. iFrame "Hγfgnpto Hℓbuf HContent".
       iPureIntro; done. }
   Qed.
 
-  Lemma bufToC_fixed ℓbuf Pb (c:nat) ℓML fid lv θ:
+  Lemma bufToC_fixed ℓbuf Pb (c:nat) ℓML γ lv θ:
       GC θ
-   -∗ isBufferRecordML (ML_lang.LitV ℓML, (ML_lang.LitV c, ML_lang.LitV (LitForeign fid))) ℓbuf Pb c
-   -∗ lv ~~ (ML_lang.LitV ℓML, (ML_lang.LitV c, ML_lang.LitV (LitForeign fid)))
+   -∗ isBufferRecordML (ML_lang.LitV ℓML, (ML_lang.LitV c, ML_lang.LitV (LitForeign γ))) ℓbuf Pb c
+   -∗ lv ~~ (ML_lang.LitV ℓML, (ML_lang.LitV c, ML_lang.LitV (LitForeign γ)))
   ==∗ GC θ ∗ isBufferRecord lv ℓbuf Pb c.
   Proof.
     iIntros "HGC H #Hsim".
     iMod (bufToC with "HGC H Hsim") as "($&$&%ℓML1&%fid1&%Href)". done.
   Qed.
 
-  Lemma bufToML_fixed lv ℓbuf Pb c (ℓML:loc) fid θ:
+  Lemma bufToML_fixed lv ℓbuf Pb c (ℓML:loc) γ θ:
       GC θ
    -∗ isBufferRecord lv ℓbuf Pb c
-   -∗ lv ~~ (ML_lang.LitV ℓML, (ML_lang.LitV c, ML_lang.LitV (LitForeign fid)))
-  ==∗ GC θ ∗ isBufferRecordML (ML_lang.LitV ℓML, (ML_lang.LitV c, ML_lang.LitV (LitForeign fid))) ℓbuf Pb c.
+   -∗ lv ~~ (ML_lang.LitV ℓML, (ML_lang.LitV c, ML_lang.LitV (LitForeign γ)))
+  ==∗ GC θ ∗ isBufferRecordML (ML_lang.LitV ℓML, (ML_lang.LitV c, ML_lang.LitV (LitForeign γ))) ℓbuf Pb c.
   Proof.
     iIntros "HGC H #Hsim".
     iMod (bufToML with "HGC H") as "(HGC&%&HML&#Hsim2)".
-    iAssert (⌜v = (ML_lang.LitV ℓML, (ML_lang.LitV c, ML_lang.LitV (LitForeign fid)))%MLV⌝)%I as "->"; last by iFrame.
+    iAssert (⌜v = (ML_lang.LitV ℓML, (ML_lang.LitV c, ML_lang.LitV (LitForeign γ)))%MLV⌝)%I as "->"; last by iFrame.
     iNamed "HML".
     cbn.
-    iDestruct "Hsim" as "#(%γ&%&%&->&Hγbuf&(%γref&->&Hsim)&%γaux&%&%&->&Hγaux&->&%γfgn2&->&Hγfgnsim2)".
-    iDestruct "Hsim2" as "#(%γ2&%&%&%HHH&Hγbuf2&(%γref2&->&Hsim2)&%γaux2&%&%&->&Hγaux2&->&%γfgn3&->&Hγfgnsim3)".
+    iDestruct "Hsim" as "#(%γ1&%&%&->&Hγbuf&(%γref&->&Hsim)&%γaux&%&%&->&Hγaux&->&->)".
+    iDestruct "Hsim2" as "#(%γ2&%&%&%HHH&Hγbuf2&(%γref2&->&Hsim2)&%γaux2&%&%&->&Hγaux2&->&->)".
     simplify_eq.
     unfold lstore_own_vblock, lstore_own_elem; cbn.
     iDestruct "Hγbuf" as "(Hγbuf&_)".
@@ -93,11 +90,9 @@ Section Specs.
     iDestruct "Hγaux2" as "(Hγaux2&_)".
     iPoseProof (ghost_map.ghost_map_elem_agree with "Hγbuf Hγbuf2") as "%Heq1"; simplify_eq.
     iPoseProof (ghost_map.ghost_map_elem_agree with "Hγaux Hγaux2") as "%Heq1"; simplify_eq.
-    iPoseProof (lloc_own_foreign_inj with "Hγfgnsim2 Hγfgnsim3 HGC") as "(HGC&%Heq1)"; simplify_eq.
     iPoseProof (lloc_own_pub_inj with "Hsim Hsim2 HGC") as "(HGC&%Heq2)"; simplify_eq.
     iPureIntro. f_equal; repeat f_equal.
     - symmetry; by eapply Heq2.
-    - symmetry; by eapply Heq1.
   Qed.
 
 End Specs.
