theories/interop/update_laws.v
@@ -219,22 +219,6 @@ Proof.
   - destruct Hχvirt as [_ [H _]]. by eapply H.
 Qed.
 
-Lemma lloc_own_foreign_inj θ γ1 γ2 fid1 fid2 :
-    γ1 ~foreign~ fid1
- -∗ γ2 ~foreign~ fid2
- -∗ GC θ
- -∗ GC θ ∗ ⌜γ1 = γ2 ↔ fid1 = fid2⌝.
-Proof.
-  iIntros "#Hsim1 #Hsim2 HGC". iNamed "HGC".
-  iPoseProof (lloc_own_foreign_of with "[$] Hsim1") as "%HH1".
-  iPoseProof (lloc_own_foreign_of with "[$] Hsim2") as "%HH2".
-  iSplit.
-  1: (repeat iExists _; iFrame; done).
-  iPureIntro; split; intros ->.
-  - by simplify_eq.
-  - destruct Hχvirt as [_ [H _]]. by eapply H.
-Qed.
-
 
 
 End UpdateLaws.
